src/dvspec/dafny/att_spec_proofs/fnc_invs_27.dfy
@@ -1812,14 +1812,15 @@ module Fnc_Invs_27
     ensures s'.rcvd_attestation_shares == s.rcvd_attestation_shares 
     { }
 
-    
+    /*
     lemma lemma_inv37_f_listen_for_attestation_shares(
         process: DVCNodeState,
         attestation_share: AttestationShare,
         process': DVCNodeState
     )
     requires f_listen_for_attestation_shares.requires(process, attestation_share)
-    requires process' == f_listen_for_attestation_shares(process, attestation_share).state       
+    requires process' == f_listen_for_attestation_shares(process, attestation_share).state     
+    
     ensures && var k := (attestation_share.data, attestation_share.aggregation_bits);
             && ( forall i, j 
                     | 
@@ -1830,7 +1831,7 @@ module Fnc_Invs_27
                                 || j != k
                              )
                              ==> 
-                             process'.rcvd_attestation_shares[i][j] == process.rcvd_attestation_shares[i][j]
+                             process'.rcvd_attestation_shares[i][j] <= process.rcvd_attestation_shares[i][j]
                            )
                         && ( ( && i == attestation_share.data.slot
                                && j == k
@@ -1851,6 +1852,7 @@ module Fnc_Invs_27
                                 <= process.rcvd_attestation_shares[i][j] + {attestation_share} 
                            )
                    )                   
+                   
     { 
         var activate_att_consensus_intances := process.attestation_consensus_engine_state.attestation_consensus_active_instances.Keys;
 
@@ -1976,7 +1978,7 @@ module Fnc_Invs_27
             assert process'.rcvd_attestation_shares == process.rcvd_attestation_shares;            
         }
     }
-    
+    */
 
     lemma lemma_inv37_f_start_next_duty(process: DVCNodeState, attestation_duty: AttestationDuty, process': DVCNodeState)
     requires f_start_next_duty.requires(process, attestation_duty)
@@ -2170,5 +2172,563 @@ module Fnc_Invs_27
         { }
     } 
 
+    lemma lemma_multicast_getMessagesFromMessagesWithRecipient(dvc: DVCNodeState, attestation_with_signature_share: AttestationShare)
+    requires |dvc.peers| > 0    
+    ensures getMessagesFromMessagesWithRecipient(multicast(attestation_with_signature_share, dvc.peers))
+            ==
+            { attestation_with_signature_share }            
+    {
+        var mcast_msgs := multicast(attestation_with_signature_share, dvc.peers);
+        assert (forall msg | msg in mcast_msgs :: msg.message == attestation_with_signature_share);
+        assert |mcast_msgs| > 0;
+        
+        var msgs_content := getMessagesFromMessagesWithRecipient(mcast_msgs);
+        
+
+        var all_mcast_msgs := mcast_msgs;
+        var checked_mcast_msgs := {};
+
+        while all_mcast_msgs != {}            
+            invariant all_mcast_msgs + checked_mcast_msgs == mcast_msgs
+            invariant checked_mcast_msgs == {}
+                        ==> getMessagesFromMessagesWithRecipient(checked_mcast_msgs) == {}
+            invariant checked_mcast_msgs != {}
+                        ==> getMessagesFromMessagesWithRecipient(checked_mcast_msgs) == { attestation_with_signature_share } 
+            decreases |all_mcast_msgs|
+        {
+            var msg :|  msg in all_mcast_msgs;
+            assert msg.message ==  attestation_with_signature_share;
+            all_mcast_msgs := all_mcast_msgs - {msg};
+            checked_mcast_msgs := checked_mcast_msgs + {msg};
+        }        
+
+        assert getMessagesFromMessagesWithRecipient(mcast_msgs) == { attestation_with_signature_share };
+    }
+
+        lemma lemma_inv38_add_block_to_bn(
+        process: DVCNodeState,
+        block: BeaconBlock,
+        process': DVCNodeState 
+    )
+    requires add_block_to_bn.requires(process, block)
+    requires process' == add_block_to_bn(process, block)    
+    ensures process'.attestation_shares_to_broadcast == process.attestation_shares_to_broadcast
+    { }
+
+    lemma lemma_inv38_f_listen_for_attestation_shares(
+        process: DVCNodeState,
+        attestation_share: AttestationShare,
+        process': DVCNodeState
+    )
+    requires f_listen_for_attestation_shares.requires(process, attestation_share)
+    requires process' == f_listen_for_attestation_shares(process, attestation_share).state       
+    ensures process'.attestation_shares_to_broadcast == process.attestation_shares_to_broadcast        
+    ensures process'.peers == process.peers          
+    { }
+
+    lemma lemma_inv38_f_start_next_duty(process: DVCNodeState, attestation_duty: AttestationDuty, process': DVCNodeState)
+    requires f_start_next_duty.requires(process, attestation_duty)
+    requires process' == f_start_next_duty(process, attestation_duty).state       
+    ensures process'.attestation_shares_to_broadcast == process.attestation_shares_to_broadcast                  
+    ensures process'.peers == process.peers
+    { } 
+
+    lemma lemma_inv38_f_resend_attestation_share(
+        process: DVCNodeState,
+        process': DVCNodeState)
+    requires f_resend_attestation_share.requires(process)
+    requires process' == f_resend_attestation_share(process).state        
+    ensures process'.attestation_shares_to_broadcast == process.attestation_shares_to_broadcast                  
+    ensures process'.peers == process.peers
+    { } 
+
+    lemma lemma_inv38_f_check_for_next_queued_duty(
+        process: DVCNodeState,
+        process': DVCNodeState
+    )
+    requires f_check_for_next_queued_duty.requires(process)
+    requires process' == f_check_for_next_queued_duty(process).state        
+    ensures process'.attestation_shares_to_broadcast == process.attestation_shares_to_broadcast                  
+    ensures process'.peers == process.peers
+    decreases process.attestation_duties_queue
+    {
+        if  && process.attestation_duties_queue != [] 
+            && (
+                || process.attestation_duties_queue[0].slot in process.future_att_consensus_instances_already_decided
+                || !process.current_attestation_duty.isPresent()
+            )    
+        {            
+                if process.attestation_duties_queue[0].slot in process.future_att_consensus_instances_already_decided.Keys 
+                {
+                    var queue_head := process.attestation_duties_queue[0];
+                    var new_attestation_slashing_db := f_update_attestation_slashing_db(process.attestation_slashing_db, process.future_att_consensus_instances_already_decided[queue_head.slot]);
+                    var process_mod := process.(
+                        attestation_duties_queue := process.attestation_duties_queue[1..],
+                        future_att_consensus_instances_already_decided := process.future_att_consensus_instances_already_decided - {queue_head.slot},
+                        attestation_slashing_db := new_attestation_slashing_db,
+                        attestation_consensus_engine_state := updateConsensusInstanceValidityCheck(
+                            process.attestation_consensus_engine_state,
+                            new_attestation_slashing_db
+                        )                        
+                    );
+
+                    assert process.attestation_slashing_db <= process_mod.attestation_slashing_db;
+                    
+                    lemma_inv38_f_check_for_next_queued_duty(process_mod, process');
+                }
+                else
+                { 
+                    var process_mod := process.(
+                        attestation_duties_queue := process.attestation_duties_queue[1..]
+                    );     
+                    assert process.attestation_slashing_db <= process_mod.attestation_slashing_db;
+                    lemma_inv38_f_start_next_duty(process_mod, process.attestation_duties_queue[0], process');
+                }
+        }
+        else
+        { }
+    }
+
+    lemma lemma_inv38_f_att_consensus_decided(
+        process: DVCNodeState,
+        id: Slot,
+        decided_attestation_data: AttestationData, 
+        process': DVCNodeState,
+        outputs: Outputs
+    )
+    requires |process.peers| > 0
+    requires f_att_consensus_decided.requires(process, id, decided_attestation_data)
+    requires process' == f_att_consensus_decided(process, id, decided_attestation_data).state         
+    requires outputs == f_att_consensus_decided(process, id, decided_attestation_data).outputs
+    // TODO: add the following precondition to f_att_consensus_decided //
+    requires process.current_attestation_duty.safe_get().slot !in process.attestation_shares_to_broadcast.Keys
+    requires decided_attestation_data.slot == process.current_attestation_duty.safe_get().slot        
+    ensures && decided_attestation_data.slot in process'.attestation_shares_to_broadcast.Keys
+            && { process'.attestation_shares_to_broadcast[decided_attestation_data.slot] }                    
+                == getMessagesFromMessagesWithRecipient(outputs.att_shares_sent)                    
+            && process'.attestation_shares_to_broadcast.Keys 
+                == process.attestation_shares_to_broadcast.Keys + {decided_attestation_data.slot}  
+            && process'.attestation_shares_to_broadcast.Values 
+                == process.attestation_shares_to_broadcast.Values 
+                        + getMessagesFromMessagesWithRecipient(outputs.att_shares_sent)  
+    {
+        
+        var local_current_attestation_duty := process.current_attestation_duty.safe_get();
+        assert local_current_attestation_duty.slot == decided_attestation_data.slot;
+
+        var attestation_slashing_db := f_update_attestation_slashing_db(process.attestation_slashing_db, decided_attestation_data);
+
+        var fork_version := bn_get_fork_version(compute_start_slot_at_epoch(decided_attestation_data.target.epoch));
+        var attestation_signing_root := compute_attestation_signing_root(decided_attestation_data, fork_version);
+        var attestation_signature_share := rs_sign_attestation(decided_attestation_data, fork_version, attestation_signing_root, process.rs);
+        var attestation_with_signature_share := AttestationShare(
+                aggregation_bits := get_aggregation_bits(local_current_attestation_duty.validator_index),
+                data := decided_attestation_data, 
+                signature := attestation_signature_share
+            ); 
+
+        var new_attestation_consensus_engine_state := updateConsensusInstanceValidityCheck(
+                                                            process.attestation_consensus_engine_state,
+                                                            attestation_slashing_db
+                                                      );
+
+        var process_mod := 
+            process.(
+                current_attestation_duty := None,
+                attestation_shares_to_broadcast := process.attestation_shares_to_broadcast[local_current_attestation_duty.slot := attestation_with_signature_share],
+                attestation_slashing_db := attestation_slashing_db,
+                attestation_consensus_engine_state := new_attestation_consensus_engine_state
+            );
+
+        assert process_mod.attestation_shares_to_broadcast.Keys 
+                == process.attestation_shares_to_broadcast.Keys + {local_current_attestation_duty.slot};
+        assert process_mod.attestation_shares_to_broadcast.Values 
+                == process.attestation_shares_to_broadcast.Values + {attestation_with_signature_share};
+        assert process_mod.peers == process.peers;
+
+
+        var new_dvc := f_check_for_next_queued_duty(process_mod).state;
+        lemma_inv38_f_check_for_next_queued_duty(process_mod, new_dvc);        
+        assert new_dvc.attestation_shares_to_broadcast == process_mod.attestation_shares_to_broadcast;
+        assert new_dvc.peers == process_mod.peers;
+        
+        var ret_dvc_outputs := DVCNodeStateAndOuputs(
+                                    state := new_dvc,
+                                    outputs := getEmptyOuputs().(
+                                        att_shares_sent := multicast(attestation_with_signature_share, new_dvc.peers)
+                                    )          
+                                );
+        
+        assert && process' == ret_dvc_outputs.state
+               && decided_attestation_data.slot in process'.attestation_shares_to_broadcast.Keys
+               && outputs == ret_dvc_outputs.outputs
+               ;     
+
+
+        lemma_multicast_getMessagesFromMessagesWithRecipient(ret_dvc_outputs.state, attestation_with_signature_share);
+
+        
+        assert { process'.attestation_shares_to_broadcast[decided_attestation_data.slot] }
+                    == { process'.attestation_shares_to_broadcast[local_current_attestation_duty.slot] }
+                    == { attestation_with_signature_share }
+                    == getMessagesFromMessagesWithRecipient(outputs.att_shares_sent);
+
+        assert { process'.attestation_shares_to_broadcast[decided_attestation_data.slot] }
+                    == getMessagesFromMessagesWithRecipient(outputs.att_shares_sent);
+
+        assert process'.attestation_shares_to_broadcast.Keys 
+                    == process.attestation_shares_to_broadcast.Keys + {decided_attestation_data.slot};
+
+        assert process'.attestation_shares_to_broadcast.Values 
+                == process.attestation_shares_to_broadcast.Values 
+                        + getMessagesFromMessagesWithRecipient(outputs.att_shares_sent);
+    }
+
+    lemma lemma_inv38_f_serve_attestation_duty(
+        process: DVCNodeState,
+        attestation_duty: AttestationDuty,
+        process': DVCNodeState
+    )  
+    requires f_serve_attestation_duty.requires(process, attestation_duty)
+    requires process' == f_serve_attestation_duty(process, attestation_duty).state
+    ensures process'.attestation_shares_to_broadcast == process.attestation_shares_to_broadcast
+    {
+        var process_mod := process.(
+                attestation_duties_queue := process.attestation_duties_queue + [attestation_duty],
+                all_rcvd_duties := process.all_rcvd_duties + {attestation_duty}
+            );        
+
+
+        lemma_inv38_f_check_for_next_queued_duty(process_mod, process');        
+    }
+
+    lemma lemma_inv38_f_listen_for_new_imported_blocks(
+        process: DVCNodeState,
+        block: BeaconBlock,
+        process': DVCNodeState
+    )
+    requires f_listen_for_new_imported_blocks.requires(process, block)
+    requires process' == f_listen_for_new_imported_blocks(process, block).state   
+    ensures process'.attestation_shares_to_broadcast.Values <= process.attestation_shares_to_broadcast.Values
+    {
+        var new_consensus_instances_already_decided := f_listen_for_new_imported_blocks_helper_1(process, block);
+
+        var att_consensus_instances_already_decided := process.future_att_consensus_instances_already_decided + new_consensus_instances_already_decided;
+
+        var future_att_consensus_instances_already_decided := 
+            f_listen_for_new_imported_blocks_helper_2(process, att_consensus_instances_already_decided);
+
+        var process :=
+                process.(
+                    future_att_consensus_instances_already_decided := future_att_consensus_instances_already_decided,
+                    attestation_consensus_engine_state := stopConsensusInstances(
+                                    process.attestation_consensus_engine_state,
+                                    att_consensus_instances_already_decided.Keys
+                    ),
+                    attestation_shares_to_broadcast := process.attestation_shares_to_broadcast - att_consensus_instances_already_decided.Keys,
+                    rcvd_attestation_shares := process.rcvd_attestation_shares - att_consensus_instances_already_decided.Keys                    
+                );    
+                
+
+        if process.current_attestation_duty.isPresent() && process.current_attestation_duty.safe_get().slot in att_consensus_instances_already_decided
+        {
+            var decided_attestation_data := att_consensus_instances_already_decided[process.current_attestation_duty.safe_get().slot];
+            var new_attestation_slashing_db := f_update_attestation_slashing_db(process.attestation_slashing_db, decided_attestation_data);
+            var new_attestation_consensus_engine_state := updateConsensusInstanceValidityCheck(
+                                                            process.attestation_consensus_engine_state,
+                                                            new_attestation_slashing_db
+                                                          );  
+            var process_mod := process.(
+                current_attestation_duty := None,
+                attestation_slashing_db := new_attestation_slashing_db,
+                attestation_consensus_engine_state := new_attestation_consensus_engine_state
+            );
+
+            
+
+            lemma_inv38_f_check_for_next_queued_duty(process_mod, process');
+        }
+        else
+        { }
+    } 
+
+    lemma lemma_inv37_f_listen_for_attestation_shares(
+        process: DVCNodeState,
+        attestation_share: AttestationShare,
+        process': DVCNodeState
+    )
+    requires f_listen_for_attestation_shares.requires(process, attestation_share)
+    requires process' == f_listen_for_attestation_shares(process, attestation_share).state         
+    ensures && var k := (attestation_share.data, attestation_share.aggregation_bits);
+            && ( forall i, j 
+                    | 
+                        && i in process'.rcvd_attestation_shares.Keys
+                        && j in process'.rcvd_attestation_shares[i].Keys
+                    :: 
+                        && ( (  || i != attestation_share.data.slot
+                                || j != k
+                             )
+                             ==> 
+                             process'.rcvd_attestation_shares[i][j] <= process.rcvd_attestation_shares[i][j]
+                           )
+                        && ( ( && i == attestation_share.data.slot
+                               && j == k
+                               && ( || i !in process.rcvd_attestation_shares.Keys 
+                                    || j !in process.rcvd_attestation_shares[i].Keys
+                                  )       
+                             )
+                             ==> 
+                             process'.rcvd_attestation_shares[i][j] <= {attestation_share} 
+                           )
+                        && ( ( && i == attestation_share.data.slot
+                               && j == k
+                               && i in process.rcvd_attestation_shares.Keys 
+                               && j in process.rcvd_attestation_shares[i].Keys                                 
+                             )
+                             ==> 
+                                process'.rcvd_attestation_shares[i][j] 
+                                <= process.rcvd_attestation_shares[i][j] + {attestation_share} 
+                           )
+                   )                                      
+    { 
+        var activate_att_consensus_intances := process.attestation_consensus_engine_state.attestation_consensus_active_instances.Keys;
+
+        if 
+            || (activate_att_consensus_intances == {} && !process.latest_attestation_duty.isPresent())
+            || (activate_att_consensus_intances != {} && minSet(activate_att_consensus_intances) <= attestation_share.data.slot)
+            || (activate_att_consensus_intances == {} && process.current_attestation_duty.isPresent() && process.current_attestation_duty.safe_get().slot <= attestation_share.data.slot)                
+            || (activate_att_consensus_intances == {} && !process.current_attestation_duty.isPresent() && process.latest_attestation_duty.isPresent() && process.latest_attestation_duty.safe_get().slot < attestation_share.data.slot)
+        {
+            var k := (attestation_share.data, attestation_share.aggregation_bits);
+            var attestation_shares_db_at_slot := getOrDefault(process.rcvd_attestation_shares, attestation_share.data.slot, map[]);
+
+            assert && ( attestation_share.data.slot in process.rcvd_attestation_shares.Keys
+                        ==> 
+                        attestation_shares_db_at_slot == process.rcvd_attestation_shares[attestation_share.data.slot]
+                      )
+                   && ( attestation_share.data.slot !in process.rcvd_attestation_shares.Keys
+                        ==> 
+                        attestation_shares_db_at_slot == map[]
+                      );
+
+            var new_set := getOrDefault(attestation_shares_db_at_slot, k, {}) + 
+                                                {attestation_share};
+
+            assert && (k in attestation_shares_db_at_slot.Keys 
+                            ==> new_set == attestation_shares_db_at_slot[k] + {attestation_share}
+                      )
+                   && (k !in attestation_shares_db_at_slot.Keys 
+                            ==> new_set == {attestation_share}
+                      );
+                
+            var new_attestation_shares_db := 
+                        process.rcvd_attestation_shares[
+                            attestation_share.data.slot := 
+                                attestation_shares_db_at_slot[
+                                            k := new_set                                                
+                                            ]
+                                ];
+
+            assert attestation_share.data.slot in new_attestation_shares_db.Keys;
+            assert k in new_attestation_shares_db[attestation_share.data.slot].Keys;
+
+            assert ( forall i, j 
+                    | 
+                        && i in new_attestation_shares_db.Keys
+                        && j in new_attestation_shares_db[i].Keys
+                    :: 
+                        && ( (  || i != attestation_share.data.slot
+                                || j != k
+                             )
+                             ==> 
+                             new_attestation_shares_db[i][j] == process.rcvd_attestation_shares[i][j]
+                           )
+                        && ( ( && i == attestation_share.data.slot
+                               && j == k
+                               && ( || i !in process.rcvd_attestation_shares.Keys 
+                                    || j !in process.rcvd_attestation_shares[i].Keys
+                                  )       
+                             )
+                             ==> 
+                             new_attestation_shares_db[i][j] == {attestation_share} 
+                           )
+                        && ( ( && i == attestation_share.data.slot
+                               && j == k
+                               && i in process.rcvd_attestation_shares.Keys 
+                               && j in process.rcvd_attestation_shares[i].Keys                                 
+                             )
+                             ==> 
+                                new_attestation_shares_db[i][j] 
+                                == process.rcvd_attestation_shares[i][j] + {attestation_share} 
+                           )
+                   )
+            ;
+
+
+            var process_mod := process.(
+                    rcvd_attestation_shares := new_attestation_shares_db
+                );
+
+            assert ( forall i, j 
+                    | 
+                        && i in process_mod.rcvd_attestation_shares.Keys
+                        && j in process_mod.rcvd_attestation_shares[i].Keys
+                    :: 
+                        && ( (  || i != attestation_share.data.slot
+                                || j != k
+                             )
+                             ==> 
+                             process_mod.rcvd_attestation_shares[i][j] == process.rcvd_attestation_shares[i][j]
+                           )
+                        && ( ( && i == attestation_share.data.slot
+                               && j == k
+                               && ( || i !in process.rcvd_attestation_shares.Keys 
+                                    || j !in process.rcvd_attestation_shares[i].Keys
+                                  )       
+                             )
+                             ==> 
+                             process_mod.rcvd_attestation_shares[i][j] == {attestation_share} 
+                           )
+                        && ( ( && i == attestation_share.data.slot
+                               && j == k
+                               && i in process.rcvd_attestation_shares.Keys
+                               && j in process.rcvd_attestation_shares[i].Keys                                 
+                             )
+                             ==> 
+                                process_mod.rcvd_attestation_shares[i][j] 
+                                == process.rcvd_attestation_shares[i][j] + {attestation_share} 
+                           )
+                   )
+            ;
+
+            if process_mod.construct_signed_attestation_signature(process_mod.rcvd_attestation_shares[attestation_share.data.slot][k]).isPresent()
+            {
+                assert process'.rcvd_attestation_shares == process_mod.rcvd_attestation_shares;            
+            }
+            else
+            {
+                assert process'.rcvd_attestation_shares == process_mod.rcvd_attestation_shares;            
+            }             
+        }
+        else
+        {             
+            assert process'.rcvd_attestation_shares == process.rcvd_attestation_shares;            
+        }
+    }
+
     
+    lemma lemma_inv37_f_listen_for_attestation_shares_domain(
+        process: DVCNodeState,
+        attestation_share: AttestationShare,
+        process': DVCNodeState
+    )
+    requires f_listen_for_attestation_shares.requires(process, attestation_share)
+    requires process' == f_listen_for_attestation_shares(process, attestation_share).state         
+    ensures && var k := (attestation_share.data, attestation_share.aggregation_bits);
+            && var slot := attestation_share.data.slot;
+            && ( forall i, j 
+                    | 
+                        || i != slot
+                        || j != k                    
+                    :: 
+                        ( && i in process'.rcvd_attestation_shares.Keys
+                          && j in process'.rcvd_attestation_shares[i].Keys               
+                        )
+                        ==>
+                        ( && i in process.rcvd_attestation_shares.Keys
+                          && j in process.rcvd_attestation_shares[i].Keys               
+                        )
+            )
+    { 
+        var activate_att_consensus_intances := process.attestation_consensus_engine_state.attestation_consensus_active_instances.Keys;
+
+        if 
+            || (activate_att_consensus_intances == {} && !process.latest_attestation_duty.isPresent())
+            || (activate_att_consensus_intances != {} && minSet(activate_att_consensus_intances) <= attestation_share.data.slot)
+            || (activate_att_consensus_intances == {} && process.current_attestation_duty.isPresent() && process.current_attestation_duty.safe_get().slot <= attestation_share.data.slot)                
+            || (activate_att_consensus_intances == {} && !process.current_attestation_duty.isPresent() && process.latest_attestation_duty.isPresent() && process.latest_attestation_duty.safe_get().slot < attestation_share.data.slot)
+        {
+            var k := (attestation_share.data, attestation_share.aggregation_bits);
+            var attestation_shares_db_at_slot := getOrDefault(process.rcvd_attestation_shares, attestation_share.data.slot, map[]);
+            var slot := attestation_share.data.slot;
+
+            assert && ( attestation_share.data.slot in process.rcvd_attestation_shares.Keys
+                        ==> 
+                        attestation_shares_db_at_slot == process.rcvd_attestation_shares[attestation_share.data.slot]
+                      )
+                   && ( attestation_share.data.slot !in process.rcvd_attestation_shares.Keys
+                        ==> 
+                        attestation_shares_db_at_slot == map[]
+                      );
+
+            var new_set := getOrDefault(attestation_shares_db_at_slot, k, {}) + 
+                                                {attestation_share};
+
+            assert && (k in attestation_shares_db_at_slot.Keys 
+                            ==> new_set == attestation_shares_db_at_slot[k] + {attestation_share}
+                      )
+                   && (k !in attestation_shares_db_at_slot.Keys 
+                            ==> new_set == {attestation_share}
+                      );
+                
+            var new_attestation_shares_db := 
+                        process.rcvd_attestation_shares[
+                            attestation_share.data.slot := 
+                                attestation_shares_db_at_slot[
+                                            k := new_set                                                
+                                            ]
+                                ];
+
+            assert attestation_share.data.slot in new_attestation_shares_db.Keys;
+            assert k in new_attestation_shares_db[attestation_share.data.slot].Keys;
+
+            assert ( forall i, j 
+                    | 
+                        || i != slot
+                        || j != k                    
+                    :: 
+                        ( && i in new_attestation_shares_db.Keys
+                          && j in new_attestation_shares_db[i].Keys               
+                        )
+                        ==>
+                        ( && i in process.rcvd_attestation_shares.Keys
+                          && j in process.rcvd_attestation_shares[i].Keys               
+                        )
+                    )
+            ;
+
+
+            var process_mod := process.(
+                    rcvd_attestation_shares := new_attestation_shares_db
+                );
+
+            assert ( forall i, j 
+                    | 
+                        || i != slot
+                        || j != k                    
+                    :: 
+                        ( && i in process_mod.rcvd_attestation_shares.Keys
+                          && j in process_mod.rcvd_attestation_shares[i].Keys               
+                        )
+                        ==>
+                        ( && i in process.rcvd_attestation_shares.Keys
+                          && j in process.rcvd_attestation_shares[i].Keys               
+                        )
+                    )
+            ;
+
+            if process_mod.construct_signed_attestation_signature(process_mod.rcvd_attestation_shares[attestation_share.data.slot][k]).isPresent()
+            {
+                assert process'.rcvd_attestation_shares == process_mod.rcvd_attestation_shares;            
+            }
+            else
+            {
+                assert process'.rcvd_attestation_shares == process_mod.rcvd_attestation_shares;            
+            }             
+        }
+        else
+        {             
+            assert process'.rcvd_attestation_shares == process.rcvd_attestation_shares;            
+        }
+    }  
 }
